module ConcreteToAbstract where

open import Prelude.Init; open SetAsType
open L.Mem
open Unary using (_âˆ©_)
open import Prelude.Lists.Membership
open import Prelude.General
open import Prelude.InferenceRules
open import Prelude.Functor
open import Prelude.FromList; open import Prelude.ToList
open import Prelude.DecEq
open import Prelude.Monad

import Prelude.Bags as B
import Prelude.Maps as M

open import Common
import UTxOErr.UTxO      as C
import ValueSepUTxO.UTxO as A
open import UTxOErr.Ledger      as C
  using ([]; _âŠ£_âˆ·_)
open import ValueSepUTxO.Ledger as A
  using ([]; _âŠ£_âˆ·_)
import ValueSepUTxO.UTxO as A
import UTxOErr.HoareLogic      as C
import ValueSepUTxO.HoareLogic as A

{- ** USE CASE

We can compositionally reason about an *abstract* UTxO ledger,
but can we transfer the results to an actual *concrete* UTxO ledger?

Well, this would only be possible for properties that do not observe the concrete
implementation details (such as the order of transaction outputs, c.f. set/list).
This could be enforced by only considering predicates of the
form: `Pá¶œ = Páµƒ âˆ˜ concreteâ†’abstract` for some abstract predicate Páµƒ and a
concreteâ†’abstract translation which forgets about implementation details.

At this point, we can use our reasoning framework on concrete ledgers,
but can we prove that this procedure is sound?
Is this even possible? Seems connected to parametricity and such...

NB: might be worth just looking at the minimal example of sets/lists and figuring
out the issue at this more simplistic setting first.
-}

M-Any-âˆ˜ : âˆ€ {A B : Type} {P : Predâ‚€ B} {f : A â†’ B} {mx : Maybe A} â†’
  M.Any.Any P (f <$> mx)
  â”€â”€â”€â”€â”€â”€â”€â”€â”€â”€â”€â”€â”€â”€â”€â”€â”€â”€â”€
  M.Any.Any (P âˆ˜ f) mx
M-Any-âˆ˜ {mx = just _} (M.Any.just p) = M.Any.just p

-- ** abstracting away implementation details
private variable
  s sâ€² : C.S
  l : C.L
  t : C.Tx

absS : C.S â†’ A.S
absS = C.valuesË¢

open â‰¡-Reasoning

postulate
  mapâˆ˜mapWithâˆˆ : âˆ€ {A B C : Type}
     (g : B â†’ C)  (xs : List A) (f : âˆ€ {x} â†’ x âˆˆ xs â†’ B)
    â†’ map g (mapWithâˆˆ xs f) â‰¡ mapWithâˆˆ xs (g âˆ˜ f)
  mapWithâˆˆâˆ˜map : âˆ€ {A B C : Type}
    (f : A â†’ B) (xs : List A) (g : âˆ€ {x} â†’ x âˆˆ map f xs â†’ C)
    â†’ mapWithâˆˆ (map f xs) g â‰¡ mapWithâˆˆ xs (g âˆ˜ âˆˆ-mapâº f)

absVT : C.IsValidTx t s â†’ âˆƒ (flip A.IsValidTx (absS s))
absVT {t}{s} vt = tÌ‚ , record
  { validOutputRefs     = vorâ€²
  ; preservesValues     = pvâ€²
  ; allInputsValidate   = L.All.tabulate aivâ€²
  ; validateValidHashes = L.All.tabulate vvhâ€² }
  module âˆ£absVTâˆ£ where
    is = t .C.inputs; os = t .C.outputs; frg = t .C.forge
    vor = vt .C.validOutputRefs

    goI : C.TxInput Ã— C.TxOutput â†’ A.TxInput
    goI (record {outputRef = _; validator = f; redeemer = r} , o)
       = record {outputRef = o; validator = f; redeemer = r}

    ris = C.resolvedInputs vt
    isâ€² = map goI ris

    tÌ‚ = record {inputs = isâ€²; outputs = os; forge = frg}
    sÌ‚ = absS s

    stxoâ‰¡ : A.stxoTx tÌ‚ â‰¡ C.valuesâŠ‘Ë¢ s (-, vor)
    stxoâ‰¡ rewrite
      begin
        A.outputRefs tÌ‚
      â‰¡Ë˜âŸ¨ L.map-compose ris âŸ©
        (A.outputRef âˆ˜ goI) <$> ris
      â‰¡âŸ¨ mapâˆ˜mapWithâˆˆ (A.outputRef âˆ˜ goI) is _ âŸ©
        mapWithâˆˆ is _
      â‰¡âŸ¨ mapWithâˆˆ-cong is _ _ (Î» _ â†’ refl) âŸ©
        mapWithâˆˆ is (C.resolved vt âˆ˜ âˆˆ-mapâº C.outputRef)
      â‰¡Ë˜âŸ¨ mapWithâˆˆâˆ˜map C.outputRef is (C.resolved vt) âŸ©
        mapWithâˆˆ (C.outputRef <$> is) (C.resolved vt)
      â‰¡âŸ¨âŸ©
        C.valuesâŠ‘ s (-, vor)
      âˆ = refl

    vorâ€² : A.stxoTx tÌ‚ B.âŠ†Ë¢ sÌ‚
    vorâ€² = subst (B._âŠ†Ë¢ C.valuesË¢ s) (sym stxoâ‰¡) (C.valuesâŠ†â‡’âŠ†Ë¢ s (-, vor))

    pvâ€² =
      begin
        tÌ‚ .A.forge + âˆ‘ (tÌ‚ .A.inputs) (value âˆ˜ A.outputRef)
      â‰¡âŸ¨âŸ©
        frg + âˆ‘ (map goI ris) (value âˆ˜ A.outputRef)
      â‰¡âŸ¨ cong (Î» â—† â†’ frg + â—†) $ cong sum $ sym $ L.map-compose ris âŸ©
        frg + âˆ‘ ris (value âˆ˜ projâ‚‚)
      â‰¡âŸ¨ vt .C.preservesValues âŸ©
        âˆ‘ os value
      â‰¡âŸ¨âŸ©
        âˆ‘ (tÌ‚ .A.outputs) value
      âˆ

    inputInfoâ‰¡ =
      begin
        (A.mkInputInfo <$> A.resolveInputs tÌ‚ (A.resolved tÌ‚))
      â‰¡âŸ¨ mapâˆ˜mapWithâˆˆ A.mkInputInfo isâ€² _ âŸ©
        mapWithâˆˆ (goI <$> ris) _
      â‰¡âŸ¨ mapWithâˆˆâˆ˜map goI ris _ âŸ©
        mapWithâˆˆ ris _
      â‰¡âŸ¨ mapWithâˆˆ-cong ris _ _ (Î» _ â†’ refl) âŸ©
        mapWithâˆˆ ris _
      â‰¡âŸ¨ mapWithâˆˆâ‰—map _ ris âŸ©
        (C.mkInputInfo <$> ris)
      âˆ

    aivâ€² : âˆ€ {i} â†’ i âˆˆ isâ€² â†’
      T $ i .A.validator (A.mkTxInfo tÌ‚ $ A.resolved tÌ‚) (i .A.redeemer)
    aivâ€² iâˆˆ
      with _ , iâˆˆ , refl â† âˆˆ-mapâ» goI iâˆˆ
      rewrite
        begin
          A.mkTxInfo tÌ‚ (A.resolved tÌ‚)
        â‰¡âŸ¨ cong (Î» â—† â†’ record {inputs = â—†; outputs = os; forge = frg}) inputInfoâ‰¡ âŸ©
          C.mkTxInfo t (C.resolved vt)
        âˆ
      with _ , iâˆˆ , refl â† âˆˆ-mapWithâˆˆâ» iâˆˆ
      = L.All.lookup (vt .C.allInputsValidate) iâˆˆ

    vvhâ€² : âˆ€ {i} â†’ i âˆˆ isâ€² â†’ i .A.outputRef .address â‰¡ i .A.validator â™¯
    vvhâ€² iâˆˆ
      with _ , iâˆˆ , refl â† âˆˆ-mapâ» goI iâˆˆ
      = L.All.lookup (vt .C.validateValidHashes) iâˆˆ

absT : C.IsValidTx t s â†’ A.Tx
absT = projâ‚ âˆ˜ absVT

postulate toâˆ˜from : toList âˆ˜ fromList {B = C.S} â‰— id

absS-âˆª : absS (s M.âˆª sâ€²) â‰¡ absS s B.âˆª absS sâ€²
absS-âˆª {s}{sâ€²} = C.valuesË¢-âˆª {m = s}{sâ€²}

absS-utxo : âˆ€ (vt : C.IsValidTx t s) â†’ absS (C.utxoTx t) â‰¡ A.utxoTx (absT vt)
absS-utxo {t}{s} vt =
  begin
    absS (fromList $ mapWithâˆˆ (t .C.outputs) (C.mkUtxo t))
  â‰¡âŸ¨âŸ©
    C.valuesË¢ (fromList $ mapWithâˆˆ (t .C.outputs) (C.mkUtxo t))
  â‰¡âŸ¨ C.valuesË¢âˆ˜fromList âŸ©
    fromList (projâ‚‚ <$> mapWithâˆˆ (t .C.outputs) (C.mkUtxo t))
  â‰¡âŸ¨ cong fromList
   $ begin
        projâ‚‚ <$> mapWithâˆˆ (t .C.outputs) (C.mkUtxo t)
      â‰¡âŸ¨ mapâˆ˜mapWithâˆˆ projâ‚‚ _ _ âŸ©
        mapWithâˆˆ (t .C.outputs) (projâ‚‚ âˆ˜ C.mkUtxo t)
      â‰¡âŸ¨ mapWithâˆˆ-cong _ _ _ (Î» _ â†’ refl) âŸ©
        mapWithâˆˆ (t .C.outputs) (Î» {o} _ â†’ o)
      â‰¡âŸ¨ mapWithâˆˆâ‰—map id _ âŸ©
        map id (t .C.outputs)
      â‰¡âŸ¨ L.map-id _ âŸ©
        t .C.outputs
      âˆ
   âŸ©
    fromList (t .C.outputs)
  â‰¡âŸ¨âŸ©
    fromList (absT vt .A.outputs)
  âˆ

absS-stxo : âˆ€ (vt : C.IsValidTx t s) â†’
  absS (s C.â”€áµË¢ C.outputRefs t) â‰¡ absS s B.â”€ A.stxoTx (absT vt)
absS-stxo {t@record{outputs = os}}{s} vt@record{validOutputRefs = vor} =
  let tÌ‚ = absT vt in
  begin
    absS (s C.â”€áµË¢ C.outputRefs t)
  â‰¡âŸ¨âŸ©
    C.valuesË¢ (s C.â”€áµË¢ C.outputRefs t)
  â‰¡âŸ¨ C.valuesË¢-â”€ vor âŸ©
    C.valuesË¢ s B.â”€ C.valuesâŠ‘Ë¢ s (-, vor)
  â‰¡Ë˜âŸ¨ cong (C.valuesË¢ s B.â”€_) $ âˆ£absVTâˆ£.stxoâ‰¡ vt âŸ©
    C.valuesË¢ s B.â”€ A.stxoTx tÌ‚
  â‰¡âŸ¨âŸ©
    absS s B.â”€ A.stxoTx tÌ‚
  âˆ

denot-abs-tâ‚€ : âˆ€ (vt : C.IsValidTx t s) â†’
  A.âŸ¦ absT vt âŸ§â‚€ (absS s) â‰¡ absS (C.âŸ¦ t âŸ§â‚€ s)
denot-abs-tâ‚€ {t}{s} vt = let tÌ‚ = absT vt in
  sym $ begin
    absS (s C.â”€áµË¢ C.outputRefs t M.âˆª C.utxoTx t)
  â‰¡âŸ¨ absS-âˆª {s C.â”€áµË¢ C.outputRefs t}{C.utxoTx t} âŸ©
    absS (s C.â”€áµË¢ C.outputRefs t) B.âˆª absS (C.utxoTx t)
  â‰¡âŸ¨ cong (B._âˆª _) (absS-stxo vt) âŸ©
    absS s B.â”€ A.stxoTx tÌ‚ B.âˆª absS (C.utxoTx t)
  â‰¡âŸ¨ cong (absS s B.â”€ A.stxoTx tÌ‚ B.âˆª_) (absS-utxo vt) âŸ©
    absS s B.â”€ A.stxoTx tÌ‚ B.âˆª A.utxoTx tÌ‚
  âˆ

denot-t : âˆ€ {t : C.Tx} {s : C.S} (vt : C.IsValidTx t s) â†’
  C.âŸ¦ t âŸ§ s â‰¡ just (C.âŸ¦ t âŸ§â‚€ s)
denot-t {t}{s} vt rewrite dec-yes (C.isValidTx? t s) vt .projâ‚‚ = refl

denot-tÌ‚ : âˆ€ {t : A.Tx} {s : A.S} (vt : A.IsValidTx t s) â†’
  A.âŸ¦ t âŸ§ s â‰¡ just (A.âŸ¦ t âŸ§â‚€ s)
denot-tÌ‚ {t}{s} vt rewrite dec-yes (A.isValidTx? t s) vt .projâ‚‚ = refl

denot-abs-t : âˆ€ {vt : C.IsValidTx t s} â†’
  A.âŸ¦ absT vt âŸ§ (absS s) â‰¡ (absS <$> C.âŸ¦ t âŸ§ s)
denot-abs-t {t}{s}{vt} =
  begin
    A.âŸ¦ absT vt âŸ§ (absS s)
  â‰¡âŸ¨ denot-tÌ‚ (absVT vt .projâ‚‚) âŸ©
    just (A.âŸ¦ absT vt âŸ§â‚€ $ absS s)
  â‰¡âŸ¨ cong just $ denot-abs-tâ‚€ vt âŸ©
    just (absS $ C.âŸ¦ t âŸ§â‚€ s)
  â‰¡Ë˜âŸ¨ M.map-just $ denot-t vt âŸ©
    (absS <$> C.âŸ¦ t âŸ§ s)
  âˆ

absVL : C.VL s l â†’ âˆƒ $ A.VL (absS s)
absVL [] = -, []
absVL {s}{.t âˆ· l} (t âŠ£ vt âˆ· vl) =
  let
    tÌ‚ , vtÌ‚ = absVT {s = s} vt
    lÌ‚  , vlÌ‚ = absVL vl

    EQ : absS (C.âŸ¦ t âŸ§â‚€ s) â‰¡ A.âŸ¦ tÌ‚ âŸ§â‚€ (absS s)
    EQ = sym $ denot-abs-tâ‚€ vt
  in
    tÌ‚ âˆ· lÌ‚ , tÌ‚ âŠ£ vtÌ‚ âˆ· subst (Î» â—† â†’ A.VL â—† lÌ‚) EQ vlÌ‚

absL : C.VL s l â†’ A.L
absL = projâ‚ âˆ˜ absVL

denot-absâ‚€ : âˆ€ (vl : C.VL s l) â†’
  A.âŸ¦ absL vl âŸ§â‚€ (absS s) â‰¡ absS (C.âŸ¦ l âŸ§â‚€ s)
denot-absâ‚€ [] = refl
denot-absâ‚€ {s} {t âˆ· l} (t âŠ£ vt âˆ· vl) = let sÌ‚ = absS s; tÌ‚ = absT vt; lÌ‚ = absL vl in
  begin
    A.âŸ¦ lÌ‚ âŸ§â‚€ (A.âŸ¦ tÌ‚ âŸ§â‚€ sÌ‚)
  â‰¡âŸ¨ cong A.âŸ¦ lÌ‚ âŸ§â‚€ $ denot-abs-tâ‚€ vt âŸ©
    A.âŸ¦ lÌ‚ âŸ§â‚€ (absS $ C.âŸ¦ t âŸ§â‚€ s)
  â‰¡âŸ¨ denot-absâ‚€ {s = C.âŸ¦ t âŸ§â‚€ s} vl âŸ©
    absS (C.âŸ¦ l âŸ§â‚€ $ C.âŸ¦ t âŸ§â‚€ s)
  âˆ

denot-l : âˆ€ {l : C.L} {s : C.S} (vl : C.VL s l) â†’
  C.âŸ¦ l âŸ§ s â‰¡ just (C.âŸ¦ l âŸ§â‚€ s)
denot-l [] = refl
denot-l (_ âŠ£ vt âˆ· vl) rewrite denot-t vt | denot-l vl = refl

denot-lÌ‚ : âˆ€ {l : A.L} {s : A.S} (vl : A.VL s l) â†’
  A.âŸ¦ l âŸ§ s â‰¡ just (A.âŸ¦ l âŸ§â‚€ s)
denot-lÌ‚ [] = refl
denot-lÌ‚ (_ âŠ£ vt âˆ· vl) rewrite denot-tÌ‚ vt | denot-lÌ‚ vl = refl

denot-abs : âˆ€ {vl : C.VL s l} â†’
  A.âŸ¦ absL vl âŸ§ (absS s) â‰¡ (absS <$> C.âŸ¦ l âŸ§ s)
denot-abs {s} {[]} {[]} = refl
denot-abs {s} {t âˆ· l} {.t âŠ£ vt âˆ· vl}
  rewrite denot-t vt | denot-tÌ‚ (absVT vt .projâ‚‚) =
  let sÌ‚ = absS s; tÌ‚ = absT vt; lÌ‚ , vlÌ‚ = absVL vl in
  begin
    A.âŸ¦ lÌ‚ âŸ§ (A.âŸ¦ tÌ‚ âŸ§â‚€ sÌ‚)
  â‰¡âŸ¨ cong A.âŸ¦ lÌ‚ âŸ§ $ denot-abs-tâ‚€ vt âŸ©
    A.âŸ¦ lÌ‚ âŸ§ (absS $ C.âŸ¦ t âŸ§â‚€ s)
  â‰¡âŸ¨ denot-lÌ‚ vlÌ‚ âŸ©
    just (A.âŸ¦ lÌ‚ âŸ§â‚€ $ absS $ C.âŸ¦ t âŸ§â‚€ s)
  â‰¡âŸ¨ cong just $ denot-absâ‚€ vl âŸ©
    just (absS $ C.âŸ¦ l âŸ§â‚€ $ C.âŸ¦ t âŸ§â‚€ s)
  â‰¡Ë˜âŸ¨ M.map-just $ denot-l vl âŸ©
    (absS <$> C.âŸ¦ l âŸ§ (C.âŸ¦ t âŸ§â‚€ s))
  âˆ

postulate
  MAny-mapâ» : âˆ€ {A B : Type} {f : A â†’ B} {mx} (P : Predâ‚€ B) â†’
    M.Any.Any P (M.map f mx)
    â”€â”€â”€â”€â”€â”€â”€â”€â”€â”€â”€â”€â”€â”€â”€â”€â”€â”€â”€â”€â”€â”€â”€â”€
    M.Any.Any (P âˆ˜ f) mx

{- ** cannot formulate soundness without relating to a specific state
soundness : âˆ€ {P Q : Predâ‚€ A.S} (vl : C.VL {!!} l) â†’
  A.âŸ¨ P âŸ© absL vl âŸ¨ Q âŸ©
  â”€â”€â”€â”€â”€â”€â”€â”€â”€â”€â”€â”€â”€â”€â”€â”€â”€â”€â”€â”€â”€â”€â”€â”€â”€â”€â”€â”€â”€
  C.âŸ¨ P âˆ˜ absS âŸ© l âŸ¨ Q âˆ˜ absS âŸ©
soundness = {!!}
-}

-- ** universally quantifying abstractt ledgers
soundness-âˆ€lÌ‚ : âˆ€ {P Q : Predâ‚€ A.S} â†’
    (âˆ€ lÌ‚ â†’ A.âŸ¨ P âŸ© lÌ‚ âŸ¨ Q âŸ©)
    â”€â”€â”€â”€â”€â”€â”€â”€â”€â”€â”€â”€â”€â”€â”€â”€â”€â”€â”€â”€â”€â”€â”€â”€â”€â”€â”€â”€â”€â”€â”€â”€â”€â”€â”€â”€â”€â”€â”€â”€â”€â”€â”€â”€â”€â”€â”€â”€â”€â”€â”€
    C.âŸ¨ (P âˆ˜ absS) âˆ© flip C.VL l âŸ© l âŸ¨ Q âˆ˜ absS âŸ©
soundness-âˆ€lÌ‚ {l}{P}{Q} PlQ {s} (Ps , vl) =
  MAny-mapâ» Q Qs
  where
    sÌ‚ = absS s
    lÌ‚ = absL vl

    QsÌ‚ : M.Any.Any Q (A.âŸ¦ lÌ‚ âŸ§ sÌ‚)
    QsÌ‚ = PlQ lÌ‚ Ps

    Qs : M.Any.Any Q (absS <$> C.âŸ¦ l âŸ§ s)
    Qs = subst (M.Any.Any Q) (denot-abs {vl = vl}) QsÌ‚

-- ** universally quantifying proofs of validity
soundness-âˆ€vl : âˆ€ {P Q : Predâ‚€ A.S} â†’
  (âˆ€ {s} (vl : C.VL s l) â†’ A.âŸ¨ P âŸ© absL vl âŸ¨ Q âŸ©)
  â”€â”€â”€â”€â”€â”€â”€â”€â”€â”€â”€â”€â”€â”€â”€â”€â”€â”€â”€â”€â”€â”€â”€â”€â”€â”€â”€â”€â”€â”€â”€â”€â”€â”€â”€â”€â”€â”€â”€â”€â”€â”€â”€â”€â”€â”€â”€â”€â”€â”€â”€
  C.âŸ¨ (P âˆ˜ absS) âˆ© flip C.VL l âŸ© l âŸ¨ Q âˆ˜ absS âŸ©
soundness-âˆ€vl {l}{P}{Q} PlQ {s} (Ps , vl) =
  MAny-mapâ» Q Qs
  where
    sÌ‚ = absS s
    lÌ‚ = absL vl

    QsÌ‚ : M.Any.Any Q (A.âŸ¦ lÌ‚ âŸ§ sÌ‚)
    QsÌ‚ = PlQ vl Ps

    Qs : M.Any.Any Q (absS <$> C.âŸ¦ l âŸ§ s)
    Qs = subst (M.Any.Any Q) (denot-abs {vl = vl}) QsÌ‚

-- ** alternative formulation using "strong" abstract Hoare triples
ğ”¸âŸ¨_âŸ©_âŠ£_âŸ¨_âŸ© : (P : Predâ‚€ A.S) (l : C.L) â†’ P âˆ˜ absS âŠ†Â¹ flip C.VL l â†’ Predâ‚€ A.S â†’ Type
ğ”¸âŸ¨ P âŸ© l âŠ£ Pâ‡’ âŸ¨ Q âŸ© =
  (âˆ€ {s} (p : (P âˆ˜ absS) s) â†’ (Q A.â†‘âˆ˜ A.âŸ¦ absL (Pâ‡’ p) âŸ§) (absS s))

semi-soundness : âˆ€ {P Q : Predâ‚€ A.S} â†’
  âˆ€ (Pâ‡’ : (P âˆ˜ absS) âŠ†Â¹ flip C.VL l) â†’
  âˆ™ ğ”¸âŸ¨ P âŸ© l âŠ£ Pâ‡’ âŸ¨ Q âŸ©
    â”€â”€â”€â”€â”€â”€â”€â”€â”€â”€â”€â”€â”€â”€â”€â”€â”€â”€â”€â”€â”€â”€â”€â”€â”€â”€â”€â”€â”€â”€â”€â”€â”€â”€â”€â”€â”€â”€â”€â”€â”€â”€â”€â”€â”€â”€â”€â”€â”€â”€â”€
    C.âŸ¨ P âˆ˜ absS âŸ© l âŸ¨ Q âˆ˜ absS âŸ©
semi-soundness {l}{P}{Q} Pâ‡’ PlQ {s} Ps
  = MAny-mapâ» Q $ subst (M.Any.Any Q) (denot-abs {vl = vl}) Qs
  where
    vl = Pâ‡’ Ps

    Qs : (Q A.â†‘âˆ˜ A.âŸ¦ absL vl âŸ§) (absS s)
    Qs = PlQ Ps


-- {P} láµƒ {Q}
-- â”€â”€â”€â”€â”€â”€â”€â”€â”€â”€â”€â”€â”€â”€â”€â”€â”€â”€â”€â”€â”€
-- {P âˆ˜ abs} conc láµƒ {Q âˆ˜ abs}

-- NB: conc either non-deterministic or canonical


{- old scribbles

abs : Predâ‚€ A.S â†’ Predâ‚€ C.S
(abs P) s = P (concreteâ†’abstract s)

-- abstraction : âˆ€ {s : A.S} (P : Predâ‚€ A.S) â†’
--   P s
--   â•â•â•â•â•â•â•
--   abs P s
-- abstraction = ?

-- ** inverse direction (aka reification)
abstractâ†’concrete : A.S â†’ C.S
abstractâ†’concrete = {!!}
  where
    goT : A.T â†’ C.Tx
    goT = {!!}

rei : Predâ‚€ C.S â†’ Predâ‚€ A.S
(rei P) s = P (abstractâ†’concrete s)

-- reification : âˆ€ {s : C.S} (P : Predâ‚€ C.S) â†’
--   P s
--   â•â•â•â•â•â•â•â•â•â•â•â•â•â•â•â•â•â•â•â•â•â•â•â•
--   P (abstractâ†’concrete s)
-- reification = ?

-- ** connecting both directions (although with abstractâˆ˜concreteâ‰—id it's trivial)
sound-abstraction : âˆ€ {s : A.S} (P : Predâ‚€ A.S) â†’
  P s
  â•â•â•â•â•â•â•â•â•â•â•â•â•â•â•â•â•â•â•â•â•â•â•â•â•â•â•â•
  abs P (abstractâ†’concrete s)
sound-abstraction = {!!}

sound-reification : âˆ€ {s : C.S} (P : Predâ‚€ C.S) â†’
  P s
  â•â•â•â•â•â•â•â•â•â•â•â•â•â•â•â•â•â•â•â•â•â•â•â•â•â•â•â•
  rei P (concreteâ†’abstract s)
sound-reification = {!!}

-- sound : âˆ€ {s : C.S} (P : Predâ‚€ A.S) â†’
--   P (concreteâ†’abstract s)

-- ** non-deterministic formulation
abstractâ†’concreteâˆ— : A.S â†’ List C.S
abstractâ†’concreteâˆ— = {!!}
  where
    goT : A.T â†’ List C.Tx
    goT = {!!}

reiâˆ— : Predâ‚€ C.S â†’ Predâ‚€ A.S
(reiâˆ— P) s = P (abstractâ†’concrete s)

-- ** relational formulation

data _-reifies-_ : C.S â†’ A.S â†’ Type where

ğ•£ei : Predâ‚€ A.S â†’ Predâ‚€ C.S
(ğ•£ei P) cs = âˆƒ Î» as â†’ (cs -reifies- as) Ã— P as

-- reificationâ€² : âˆ€ {ss : A.S} {cs : C.S} (P : Predâ‚€ C.S)
--   â†’ cs -reifies- as
--   â†’ P s â†” (ğ•£ei P) cs
-- reificationâ€² = ?
-}
